Computation.v
@@ -67,7 +67,6 @@ Section comp.
     Proof.
       destruct 1; eauto.
     Qed.
-<<<<<<< variant A
 
     Section CompInv.
       (** Lifting Properties on [A] to Computations on [A] **)
@@ -112,53 +111,6 @@ Section comp.
 
   End CompInv.
 
->>>>>>> variant B
-
-    Section CompInv.
-      (** Lifting Properties on [A] to Computations on [A] **)
-
-      (* Computation preserves invariants. *)
-      Definition computational_inv A (P : Ensemble A) c :=
-        forall v, computes_to c v -> P v.
-
-      (* Relation to assist in building proofs of compuational_inv *)
-      Inductive CompInv : forall {A : Type}, Ensemble A -> Comp A -> Prop :=
-      | Return_Inv : forall A (a : A) (P : Ensemble A),
-                       P a -> CompInv P (Return a)
-      | Bind_Inv : forall A B (PA : Ensemble A) (PB : Ensemble B) comp_a comp_f,
-                     CompInv PA comp_a ->
-                     (forall (a : A), PA a -> CompInv PB (comp_f a)) ->
-                     CompInv PB (Bind comp_a comp_f)
-      | Pick_Inv : forall A (P P' : Ensemble A),
-                     (forall a, P a -> P' a) -> CompInv P' (Pick P).
-
-      Lemma CompInv_inv A c (P : Ensemble A)
-      : CompInv P c -> match c with
-                         | Return A x => fun P => P x
-                         | Bind A B x f => fun PB => exists PA : Ensemble A,
-                                                       CompInv PA x /\
-                                                       forall b : A, PA b -> CompInv PB (f b)
-                         | Pick A P => fun P' => (forall a, P a -> P' a)
-                       end P.
-      Proof.
-        destruct 1; eauto.
-      Qed.
-
-      Arguments computational_inv A P c / .
-
-      Lemma CompInv_compuational_inv A (P : Ensemble A) c
-      : CompInv P c -> computational_inv P c.
-      Proof.
-        induction c; intros; apply_in_hyp_no_cbv_match CompInv_inv; simpl;
-        intros; apply_in_hyp_no_cbv_match computes_to_inv; subst; eauto.
-        destruct_ex; split_and; simpl in *;
-        eapply H; eauto; eapply H4; eapply IHc; eauto.
-      Qed.
-
-  End CompInv.
-
-####### Ancestor
-======= end
   End computes_to.
 
   Section is_computational.
